%!Mode:: "TeX:UTF-8"
%!TEX encoding = UTF-8 Unicode
%!TEX TS-program = xelatex × 2
\documentclass{ctexart}
\newif\ifpreface
%\prefacetrue
\input{../../../global/all}
\begin{document}
\large
\setlength{\baselineskip}{1.2em}
\ifpreface
    \input{../../../global/preface}
    \newgeometry{left=2cm,right=2cm,top=2cm,bottom=2cm}
\else
\newgeometry{left=2cm,right=2cm,top=2cm,bottom=2cm}
\maketitle
\fi

%from_here_to_type
\begin{problem}
    proof: $\sum_{i=0}^{\infty}(-1)^i\Cb{n+i}{i}x^i=\frac{1}{(1+x)^{n+1}}$
\end{problem}
\begin{solution}
    \begin{enumerate}
        \item $n=0$: obviously!
        \item Assume $n$, we have the equation.
        \item We go to $n+1$, so $
                \frac{1}{(1+x)^{n+2}}=\frac{1}{(1+x)^{n+1}}\frac{1}{1+x}
                =\sum_{i=0}^{\infty}(-1)^i\Cb{n+i}{i}x^i\sum_{i=0}^{\infty}(-1)^ix^i=\sum_{i=0}^{\infty}(-1)^i\sum_{l=0}^i\Cb{n+l}{l}x^i=\sum_{i=0}^{\infty}(-1)^i\Cb{n+i+1}{i}x^i$

    \end{enumerate}
\end{solution}

\begin{problem}
    Power series expansion: $\frac{2+3x-6x^2}{1-2x}$.
\end{problem}
\begin{solution}
Let $t=2x$, so $\frac{2+3x-6x^2}{1-2x}=\frac{1}{2}\frac{4+3t-3t^2}{1-t}=\frac{2}{1-t}+\frac{3t}{2}=2\sum_{i=0}^{\infty}t^i+\frac{3t}{2}=2+\frac{7}{2}t+2\sum_{i=2}^{\infty}t^i=2+7x+\sum_{i=2}^{\infty}2^{i+1}x^i$.
\end{solution}

\end{document}